# Generalized_damage_model
### Equation 1: Elasticity
`σ = (1 - D) * C : (ε_total - ε_pl - ε_cr)`

### Equation 2: Yield Condition
`Φ_pl = √(3/2 (s_eff - X):(s_eff - X)) - [σ_y0 + R] = 0`

### Equation 3: Creep Integration (Modified Norton)
`Φ_cr = ε_cr - ε_cr₀ - Δt * (3/2) * A * (σ_eff)^(n-1) * s * (ε_cr_eqv)^q = 0`

### Equation 4: Equivalent Creep Strain Integration (Modified Norton)
`Φ_cr_eqv = ε_cr_eqv - ε_cr_eqv₀ - Δt * A * (σ_eff)^n * (ε_cr_eqv)^q = 0`

### Equation 5: Plastic Damage Integration
`Φ_Dpl = D_pl - D_pl₀ - Δt * (Y/S)^s * (Δε_pl_eqv/Δt) * (1 - D)^(-k) = 0`

### Equation 6: Creep Damage Integration
`Φ_Dcr = D_cr - D_cr₀ - Δt * A_cr * (σ_eff)^r = 0`

### Equation 7: Kinematic Hardening Integration (Chaboche)
`Φ_X1 = X1 - X1₀ - (2/3) * C1_X * (ε_pl - ε_pl₀) + γ1_X * X * (ε_pl_eqv - ε_pl_eqv₀) = 0`

### Equation 8: Kinematic Hardening Integration (Chaboche)
`Φ_X2 = X2 - X2₀ - (2/3) * C2_X * (ε_pl - ε_pl₀) + γ2_X * X * (ε_pl_eqv - ε_pl_eqv₀) = 0`

### Equation 9: Kinematic Hardening Integration (Chaboche)
`Φ_X3 = X3 - X3₀ - (2/3) * C3_X * (ε_pl - ε_pl₀) + γ3_X * X * (ε_pl_eqv - ε_pl_eqv₀) = 0`

### Equation 10: Isotropic Hardening Integration (Power law)
`Φ_R = R - K * (ε_pl_eqv)^m = 0`

### Equation 11: Plastic Strain Definition
`Φ_flow = ε_pl - ε_pl₀ - Δλ * (3/2) * (s_eff - X) / √(3/2 (s_eff - X):(s_eff - X)) = 0`

### Equation 12: Hardening Parameter Relation
`Φ_alpha = ε_pl_eqv - ε_pl_eqv₀ - Δλ = 0`

**In this system:**  
- `σ` - Stress tensor  
- `ε_pl` - Plastic strain tensor  
- `ε_cr` - Creep strain tensor  
- `ε_cr_eqv` - Equivalent creep strain (scalar)  
- `ε_pl_eqv` - Equivalent plastic strain (scalar)  
- `X = X1 + X2 + X3` - Total backstress tensor  
- `R` - Yield surface radius (scalar)  
- `λ` - Plastic multiplier (scalar)  
- `X` - Deviatoric backstress tensor  
- `D = D_pl + D_cr - D_cr*D_pl` - Total damage measure (scalar)  
- `D_pl` - Plastic damage (scalar)  
- `D_cr` - Creep damage (scalar)  
- `σ_eff = σ / (1 - D)` - Effective stress tensor  
- `s_eff = s / (1 - D)` - Effective stress deviator tensor  
- `C` - Elasticity tensor (4th rank)  
- `Y = (σ_eff²) / (2E(1-D_pl)²) * [2/3*(1+ν) + 3(1-2ν) * (σ_H/σ_eff)²]`  
- `σ_H` - Hydrostatic stress